src/program_proof/pav/logical_audit.v
@@ -4,31 +4,17 @@ From Perennial.program_proof.pav Require Import core serde merkle.
 Section proof.
 Context `{!heapGS Σ, !pavG Σ}.
 
-Definition mono_maps (ms : list adtr_map_ty) :=
+Definition mono_maps (ms : list merkle_map_ty) :=
   ∀ (i j : w64) mi mj,
   ms !! (uint.nat i) = Some mi →
   ms !! (uint.nat j) = Some mj →
   uint.Z i ≤ uint.Z j →
   mi ⊆ mj.
 
-Definition ok_epochs (ms : list adtr_map_ty) :=
-  ∀ (ep : w64) m_ep k ep' comm,
-  ms !! (uint.nat ep) = Some m_ep →
-  m_ep !! k = Some (ep', comm) →
-  uint.Z ep' ≤ uint.Z ep.
-
-(* TODO: maybe change adtr_map_ty to have MapValPre instead of pair. *)
-Definition map_lower (higher : adtr_map_ty) (lower : merkle_map_ty) :=
-  map_Forall2 (λ _ x y, MapValPre.encodes x y) lower
-    ((λ x, MapValPre.mk x.1 x.2) <$> higher).
-
-Definition audit_gs_inv (gs : list (adtr_map_ty * dig_ty)) : iProp Σ :=
+Definition audit_gs_inv (gs : list (merkle_map_ty * dig_ty)) : iProp Σ :=
   "#His_digs" ∷ ([∗ list] x ∈ gs,
-    ∃ lower,
-    "%Hlower" ∷ ⌜ map_lower x.1 lower ⌝ ∗
-    "#His_map" ∷ is_merkle_map lower x.2) ∗
-  "%Hmono_maps" ∷ ⌜ mono_maps gs.*1 ⌝ ∗
-  "%Hok_epochs" ∷ ⌜ ok_epochs gs.*1 ⌝.
+    "#His_map" ∷ is_merkle_map x.1 x.2) ∗
+  "%Hmono_maps" ∷ ⌜ mono_maps gs.*1 ⌝.
 
 Definition sigpred γ : (list w8 → iProp Σ) :=
   λ preByt,
@@ -38,20 +24,18 @@ Definition sigpred γ : (list w8 → iProp Σ) :=
   "%Hlook_dig" ∷ ⌜ gs !! uint.nat pre.(PreSigDig.Epoch) = Some (m, pre.(PreSigDig.Dig)) ⌝ ∗
   "#Hinv_gs" ∷ audit_gs_inv gs)%I.
 
-Lemma audit_gs_snoc gs upd lowered_new_map dig :
+Lemma audit_gs_snoc gs upd dig :
   let new_map := (upd ∪ (default ∅ (last gs.*1))) in
   upd ##ₘ (default ∅ (last gs.*1)) →
-  map_lower new_map lowered_new_map →
-  map_Forall (λ _ v, v.1 = W64 (length gs)) upd →
   audit_gs_inv gs -∗
-  is_merkle_map lowered_new_map dig -∗
+  is_merkle_map new_map dig -∗
   audit_gs_inv (gs ++ [(new_map, dig)]).
 Proof.
-  simpl. iIntros (Hdisj Hlower Hok_epoch) "#Hold_inv #His_dig".
+  simpl. iIntros (Hdisj) "#Hold_inv #His_dig".
   iNamedSuffix "Hold_inv" "_old".
-  iSplit; [|iPureIntro; split].
+  iSplit.
   - iApply big_sepL_snoc. iFrame "#%".
-  - unfold mono_maps in *. intros * Hlook_gsi Hlook_gsj Heq_ep.
+  - iPureIntro. unfold mono_maps in *. intros * Hlook_gsi Hlook_gsj Heq_ep.
     rewrite fmap_app in Hlook_gsi Hlook_gsj.
     destruct (decide (uint.Z i = uint.Z j)).
     { by simplify_eq/=. }
@@ -77,23 +61,6 @@ Proof.
       (W64 (pred $ length gs)) _ _ Hlook_gsi _ _); [|word].
     replace (uint.nat (W64 _)) with (pred $ length gs); [|word].
     by rewrite length_fmap in Hlast.
-  - unfold ok_epochs in *. intros * Hlook_gs Hlook_m.
-    rewrite fmap_app in Hlook_gs.
-    destruct (decide (uint.Z ep < length gs)).
-    { eapply Hok_epochs_old; [|done].
-      rewrite lookup_app_l in Hlook_gs; [done|].
-      rewrite length_fmap. word. }
-    rewrite lookup_app_r in Hlook_gs.
-    2: { rewrite length_fmap. word. }
-    simpl in *. apply list_lookup_singleton_Some in Hlook_gs as [Heq_ep <-].
-    apply lookup_union_Some_raw in Hlook_m as [Hlook_upd | [_ Hlook_last]].
-    { pose proof (map_Forall_lookup_1 _ _ _ _ Hok_epoch Hlook_upd) as ?.
-      simpl in *. subst. word. }
-    destruct (last gs.*1) as [m_last|] eqn:Hlast; [|set_solver]. simpl in *.
-    opose proof (Hok_epochs_old
-      (W64 (pred $ length gs)) _ _ _ _ _ Hlook_last) as ?; [|word].
-    replace (uint.nat (W64 _)) with (pred $ length gs); [|word].
-    by rewrite last_lookup length_fmap in Hlast.
 Qed.
 
 Lemma audit_gs_prefix l l' :
@@ -101,18 +68,14 @@ Lemma audit_gs_prefix l l' :
   audit_gs_inv l -∗
   audit_gs_inv l'.
 Proof.
-  iIntros (Hpref). iNamed 1. iSplit; [|iPureIntro; split].
+  iIntros (Hpref). iNamed 1. iSplit.
   - opose proof (prefix_to_take _ _ Hpref) as ->.
     by iApply big_sepL_take.
-  - intros ???? Hlook0 Hlook1 ?.
+  - iPureIntro. intros ???? Hlook0 Hlook1 ?.
     apply (prefix_fmap fst) in Hpref.
     opose proof (prefix_lookup_Some _ _ _ _ Hlook0 Hpref) as Hlook0'.
     opose proof (prefix_lookup_Some _ _ _ _ Hlook1 Hpref) as Hlook1'.
     by apply (Hmono_maps _ _ _ _ Hlook0' Hlook1').
-  - intros ????? Hlook0 Hlook1.
-    apply (prefix_fmap fst) in Hpref.
-    opose proof (prefix_lookup_Some _ _ _ _ Hlook0 Hpref) as Hlook0'.
-    by apply (Hok_epochs _ _ _ _ _ Hlook0' Hlook1).
 Qed.
 
 End proof.
